backends/lean/Aeneas/Std/Scalar/Ops/Sub.lean
@@ -37,12 +37,12 @@ instance {ty} : HSub (IScalar ty) (IScalar ty) (Result (IScalar ty)) where
 -/
 
 theorem UScalar.sub_equiv {ty} (x y : UScalar ty) :
-  match x - y with
-  | ok z =>
+  match (x - y).match with
+  | .ok z =>
     y.val ≤ x.val ∧
     x.val = z.val + y.val ∧
     z.bv = x.bv - y.bv
-  | fail _ => x.val < y.val
+  | .vis (.fail _) _ => x.val < y.val
   | _ => ⊥ := by
   have : x - y = sub x y := by rfl
   simp [this, sub]
@@ -81,12 +81,12 @@ theorem UScalar.sub_equiv {ty} (x y : UScalar ty) :
     ring_nf
 
 theorem IScalar.sub_equiv {ty} (x y : IScalar ty) :
-  match x - y with
-  | ok z =>
+  match (x - y).match with
+  | .ok z =>
     IScalar.inBounds ty (x.val - y.val) ∧
     z.val = x.val - y.val ∧
     z.bv = x.bv - y.bv
-  | fail _ => ¬ (IScalar.inBounds ty (x.val - y.val))
+  | .vis (.fail _) _ => ¬ (IScalar.inBounds ty (x.val - y.val))
   | _ => ⊥ := by
   have : x - y = sub x y := by rfl
   simp [this, sub]
