backends/lean/Aeneas/Std/Vec.lean
@@ -210,11 +210,8 @@ theorem Vec.set_length {α : Type u} (v: Vec α) (i: Usize) (x: α) :
 
 def Vec.index_mut_usize {α : Type u} (v: Vec α) (i: Usize) :
   Result (α × (α → Vec α)) :=
-  match Vec.index_usize v i with
-  | ok x =>
-    ok (x, Vec.set v i)
-  | fail e => fail e
-  | div => div
+  do let x ← Vec.index_usize v i
+     ok (x, Vec.set v i)
 
 @[step]
 theorem Vec.index_mut_usize_spec {α : Type u} (v: Vec α) (i: Usize)
@@ -267,6 +264,12 @@ theorem Vec.index_mut_slice_index {α : Type} (v : Vec α) (i : Usize) :
   Vec.index_mut (core.slice.index.SliceIndexUsizeSlice α) v i =
   index_mut_usize v i := by
   simp [Vec.index_mut, Vec.index_mut_usize, Slice.index_mut_usize]
+  apply congrArg (fun k => bind (v.slice.index_usize i) k)
+  funext x
+  simp [Functor.map]
+  funext x'
+  apply Vec.ext
+  simp [Vec.set, Vec.from, Slice.set, Slice.setAtNat]
   rfl
 
 -- Vec index/index_mut with RangeTo
@@ -400,11 +403,14 @@ def alloc.vec.Vec.with_capacity (T : Type) (_ : Usize) : alloc.vec.Vec T := Vec.
 def alloc.vec.Vec.extend_from_slice {T : Type} (cloneInst : core.clone.Clone T)
   (v : alloc.vec.Vec T) (s : Slice T) : Result (alloc.vec.Vec T) :=
   if h : v.length + s.length ≤ Usize.max then do
-    match h' : Slice.clone cloneInst.clone s with
-    | ok s' =>
-      ok (.from (v.val ++ s'.val) (by have := Slice.clone_length h'; scalar_tac))
-    | fail e => fail e
-    | div => div
+    match h' : (Slice.clone cloneInst.clone s).match with
+    | .ok s' =>
+      ok (.from (v.val ++ s'.val) (by
+        simp at h'
+        have := Slice.clone_length h'
+        scalar_tac))
+    | .vis eff k => Result.vis eff (fun x => nomatch x)
+    | .div => div
   else fail .panic
 
 @[rust_fun "alloc::vec::{core::ops::deref::Deref<alloc::vec::Vec<@T>, [@T]>}::deref"
