tests/lean/IterAdapters.lean
@@ -52,7 +52,7 @@ def test_enumerate_slice : Result Unit := do
   massert b
 
 /- Unit test for [iter_adapters::test_enumerate_slice] -/
-#assert (test_enumerate_slice == ok ())
+#assert (test_enumerate_slice).reducesTo ()
 
 /-- [iter_adapters::test_enumerate_empty]:
     Source: 'tests/src/iter_adapters.rs', lines 28:0-32:1
@@ -70,7 +70,7 @@ def test_enumerate_empty : Result Unit := do
   massert b
 
 /- Unit test for [iter_adapters::test_enumerate_empty] -/
-#assert (test_enumerate_empty == ok ())
+#assert (test_enumerate_empty).reducesTo ()
 
 /-- [iter_adapters::test_take_2]:
     Source: 'tests/src/iter_adapters.rs', lines 40:0-46:1
@@ -100,7 +100,7 @@ def test_take_2 : Result Unit := do
   massert b
 
 /- Unit test for [iter_adapters::test_take_2] -/
-#assert (test_take_2 == ok ())
+#assert (test_take_2).reducesTo ()
 
 /-- [iter_adapters::test_take_0]:
     Source: 'tests/src/iter_adapters.rs', lines 50:0-54:1
@@ -119,7 +119,7 @@ def test_take_0 : Result Unit := do
   massert b
 
 /- Unit test for [iter_adapters::test_take_0] -/
-#assert (test_take_0 == ok ())
+#assert (test_take_0).reducesTo ()
 
 /-- [iter_adapters::test_take_more_than_available]:
     Source: 'tests/src/iter_adapters.rs', lines 58:0-65:1
@@ -152,7 +152,7 @@ def test_take_more_than_available : Result Unit := do
   massert b
 
 /- Unit test for [iter_adapters::test_take_more_than_available] -/
-#assert (test_take_more_than_available == ok ())
+#assert (test_take_more_than_available).reducesTo ()
 
 /-- [iter_adapters::test_range_u8]: loop body 0:
     Source: 'tests/src/iter_adapters.rs', lines 75:4-77:5
@@ -187,7 +187,7 @@ def test_range_u8 : Result Unit := do
   massert (count = 5#u32)
 
 /- Unit test for [iter_adapters::test_range_u8] -/
-#assert (test_range_u8 == ok ())
+#assert (test_range_u8).reducesTo ()
 
 /-- [iter_adapters::test_range_u16]: loop body 0:
     Source: 'tests/src/iter_adapters.rs', lines 85:4-87:5
@@ -224,7 +224,7 @@ def test_range_u16 : Result Unit := do
   massert (count = 4#u32)
 
 /- Unit test for [iter_adapters::test_range_u16] -/
-#assert (test_range_u16 == ok ())
+#assert (test_range_u16).reducesTo ()
 
 /-- [iter_adapters::test_range_u32]: loop body 0:
     Source: 'tests/src/iter_adapters.rs', lines 95:4-97:5
@@ -261,7 +261,7 @@ def test_range_u32 : Result Unit := do
   massert (count = 3#u32)
 
 /- Unit test for [iter_adapters::test_range_u32] -/
-#assert (test_range_u32 == ok ())
+#assert (test_range_u32).reducesTo ()
 
 /-- [iter_adapters::test_range_u64]: loop body 0:
     Source: 'tests/src/iter_adapters.rs', lines 105:4-107:5
@@ -298,7 +298,7 @@ def test_range_u64 : Result Unit := do
   massert (count = 4#u64)
 
 /- Unit test for [iter_adapters::test_range_u64] -/
-#assert (test_range_u64 == ok ())
+#assert (test_range_u64).reducesTo ()
 
 /-- [iter_adapters::test_range_usize]: loop body 0:
     Source: 'tests/src/iter_adapters.rs', lines 115:4-117:5
@@ -337,7 +337,7 @@ def test_range_usize : Result Unit := do
   massert (count = 5#usize)
 
 /- Unit test for [iter_adapters::test_range_usize] -/
-#assert (test_range_usize == ok ())
+#assert (test_range_usize).reducesTo ()
 
 /-- [iter_adapters::test_range_empty]: loop body 0:
     Source: 'tests/src/iter_adapters.rs', lines 125:4-127:5
@@ -372,7 +372,7 @@ def test_range_empty : Result Unit := do
   massert (count = 0#u32)
 
 /- Unit test for [iter_adapters::test_range_empty] -/
-#assert (test_range_empty == ok ())
+#assert (test_range_empty).reducesTo ()
 
 /-- [iter_adapters::test_array_into_iter]:
     Source: 'tests/src/iter_adapters.rs', lines 137:0-144:1
@@ -395,7 +395,7 @@ def test_array_into_iter : Result Unit := do
   massert b
 
 /- Unit test for [iter_adapters::test_array_into_iter] -/
-#assert (test_array_into_iter == ok ())
+#assert (test_array_into_iter).reducesTo ()
 
 /-- [iter_adapters::test_slice_into_iter]:
     Source: 'tests/src/iter_adapters.rs', lines 148:0-157:1
@@ -421,7 +421,7 @@ def test_slice_into_iter : Result Unit := do
   massert b
 
 /- Unit test for [iter_adapters::test_slice_into_iter] -/
-#assert (test_slice_into_iter == ok ())
+#assert (test_slice_into_iter).reducesTo ()
 
 /-- [iter_adapters::test_enumerate_step_by]:
     Source: 'tests/src/iter_adapters.rs', lines 165:0-172:1
@@ -454,7 +454,7 @@ def test_enumerate_step_by : Result Unit := do
   massert (x1 = 30#u32)
 
 /- Unit test for [iter_adapters::test_enumerate_step_by] -/
-#assert (test_enumerate_step_by == ok ())
+#assert (test_enumerate_step_by).reducesTo ()
 
 /-- [iter_adapters::test_enumerate_take]:
     Source: 'tests/src/iter_adapters.rs', lines 176:0-184:1
@@ -493,7 +493,7 @@ def test_enumerate_take : Result Unit := do
   massert b
 
 /- Unit test for [iter_adapters::test_enumerate_take] -/
-#assert (test_enumerate_take == ok ())
+#assert (test_enumerate_take).reducesTo ()
 
 /-- [iter_adapters::test_take_exhausted_then_next]:
     Source: 'tests/src/iter_adapters.rs', lines 188:0-197:1
@@ -521,7 +521,7 @@ def test_take_exhausted_then_next : Result Unit := do
   massert b1
 
 /- Unit test for [iter_adapters::test_take_exhausted_then_next] -/
-#assert (test_take_exhausted_then_next == ok ())
+#assert (test_take_exhausted_then_next).reducesTo ()
 
 /-- [iter_adapters::test_range_single_element]:
     Source: 'tests/src/iter_adapters.rs', lines 206:0-210:1
@@ -537,7 +537,7 @@ def test_range_single_element : Result Unit := do
   massert b
 
 /- Unit test for [iter_adapters::test_range_single_element] -/
-#assert (test_range_single_element == ok ())
+#assert (test_range_single_element).reducesTo ()
 
 /-- [iter_adapters::test_range_u8_near_max]:
     Source: 'tests/src/iter_adapters.rs', lines 214:0-218:1
@@ -553,7 +553,7 @@ def test_range_u8_near_max : Result Unit := do
   massert b
 
 /- Unit test for [iter_adapters::test_range_u8_near_max] -/
-#assert (test_range_u8_near_max == ok ())
+#assert (test_range_u8_near_max).reducesTo ()
 
 /-- [iter_adapters::test_range_u8_start_gt_end]:
     Source: 'tests/src/iter_adapters.rs', lines 222:0-225:1
@@ -566,7 +566,7 @@ def test_range_u8_start_gt_end : Result Unit := do
   massert b
 
 /- Unit test for [iter_adapters::test_range_u8_start_gt_end] -/
-#assert (test_range_u8_start_gt_end == ok ())
+#assert (test_range_u8_start_gt_end).reducesTo ()
 
 /-- [iter_adapters::test_range_u8_start_eq_end]:
     Source: 'tests/src/iter_adapters.rs', lines 229:0-232:1
@@ -579,7 +579,7 @@ def test_range_u8_start_eq_end : Result Unit := do
   massert b
 
 /- Unit test for [iter_adapters::test_range_u8_start_eq_end] -/
-#assert (test_range_u8_start_eq_end == ok ())
+#assert (test_range_u8_start_eq_end).reducesTo ()
 
 /-- [iter_adapters::test_range_u16_boundary]:
     Source: 'tests/src/iter_adapters.rs', lines 236:0-242:1
@@ -604,7 +604,7 @@ def test_range_u16_boundary : Result Unit := do
   massert b
 
 /- Unit test for [iter_adapters::test_range_u16_boundary] -/
-#assert (test_range_u16_boundary == ok ())
+#assert (test_range_u16_boundary).reducesTo ()
 
 /-- [iter_adapters::test_range_u32_boundary]:
     Source: 'tests/src/iter_adapters.rs', lines 246:0-251:1
@@ -625,7 +625,7 @@ def test_range_u32_boundary : Result Unit := do
   massert b
 
 /- Unit test for [iter_adapters::test_range_u32_boundary] -/
-#assert (test_range_u32_boundary == ok ())
+#assert (test_range_u32_boundary).reducesTo ()
 
 /-- [iter_adapters::test_range_u64_boundary]:
     Source: 'tests/src/iter_adapters.rs', lines 255:0-261:1
@@ -650,7 +650,7 @@ def test_range_u64_boundary : Result Unit := do
   massert b
 
 /- Unit test for [iter_adapters::test_range_u64_boundary] -/
-#assert (test_range_u64_boundary == ok ())
+#assert (test_range_u64_boundary).reducesTo ()
 
 /-- [iter_adapters::test_range_usize_start_gt_end]:
     Source: 'tests/src/iter_adapters.rs', lines 265:0-268:1
@@ -663,7 +663,7 @@ def test_range_usize_start_gt_end : Result Unit := do
   massert b
 
 /- Unit test for [iter_adapters::test_range_usize_start_gt_end] -/
-#assert (test_range_usize_start_gt_end == ok ())
+#assert (test_range_usize_start_gt_end).reducesTo ()
 
 /-- [iter_adapters::test_step_by_larger_than_range]:
     Source: 'tests/src/iter_adapters.rs', lines 272:0-276:1
@@ -685,7 +685,7 @@ def test_step_by_larger_than_range : Result Unit := do
   massert b
 
 /- Unit test for [iter_adapters::test_step_by_larger_than_range] -/
-#assert (test_step_by_larger_than_range == ok ())
+#assert (test_step_by_larger_than_range).reducesTo ()
 
 /-- [iter_adapters::test_step_by_exact_range]:
     Source: 'tests/src/iter_adapters.rs', lines 280:0-284:1
@@ -707,7 +707,7 @@ def test_step_by_exact_range : Result Unit := do
   massert b
 
 /- Unit test for [iter_adapters::test_step_by_exact_range] -/
-#assert (test_step_by_exact_range == ok ())
+#assert (test_step_by_exact_range).reducesTo ()
 
 /-- [iter_adapters::test_step_by_one]:
     Source: 'tests/src/iter_adapters.rs', lines 288:0-295:1
@@ -744,7 +744,7 @@ def test_step_by_one : Result Unit := do
   massert b
 
 /- Unit test for [iter_adapters::test_step_by_one] -/
-#assert (test_step_by_one == ok ())
+#assert (test_step_by_one).reducesTo ()
 
 /-- [iter_adapters::test_step_by_empty]:
     Source: 'tests/src/iter_adapters.rs', lines 299:0-302:1
@@ -761,7 +761,7 @@ def test_step_by_empty : Result Unit := do
   massert b
 
 /- Unit test for [iter_adapters::test_step_by_empty] -/
-#assert (test_step_by_empty == ok ())
+#assert (test_step_by_empty).reducesTo ()
 
 /-- [iter_adapters::test_step_by_odd_range]:
     Source: 'tests/src/iter_adapters.rs', lines 306:0-312:1
@@ -793,7 +793,7 @@ def test_step_by_odd_range : Result Unit := do
   massert b
 
 /- Unit test for [iter_adapters::test_step_by_odd_range] -/
-#assert (test_step_by_odd_range == ok ())
+#assert (test_step_by_odd_range).reducesTo ()
 
 /-- [iter_adapters::test_step_by_u8_near_max]:
     Source: 'tests/src/iter_adapters.rs', lines 316:0-322:1
@@ -825,7 +825,7 @@ def test_step_by_u8_near_max : Result Unit := do
   massert b
 
 /- Unit test for [iter_adapters::test_step_by_u8_near_max] -/
-#assert (test_step_by_u8_near_max == ok ())
+#assert (test_step_by_u8_near_max).reducesTo ()
 
 /-- [iter_adapters::test_range_inclusive_basic]:
     Source: 'tests/src/iter_adapters.rs', lines 330:0-336:1
@@ -854,7 +854,7 @@ def test_range_inclusive_basic : Result Unit := do
   massert b
 
 /- Unit test for [iter_adapters::test_range_inclusive_basic] -/
-#assert (test_range_inclusive_basic == ok ())
+#assert (test_range_inclusive_basic).reducesTo ()
 
 /-- [iter_adapters::test_range_inclusive_singleton]:
     Source: 'tests/src/iter_adapters.rs', lines 340:0-344:1
@@ -873,7 +873,7 @@ def test_range_inclusive_singleton : Result Unit := do
   massert b
 
 /- Unit test for [iter_adapters::test_range_inclusive_singleton] -/
-#assert (test_range_inclusive_singleton == ok ())
+#assert (test_range_inclusive_singleton).reducesTo ()
 
 /-- [iter_adapters::test_range_inclusive_empty]:
     Source: 'tests/src/iter_adapters.rs', lines 348:0-351:1
@@ -887,6 +887,6 @@ def test_range_inclusive_empty : Result Unit := do
   massert b
 
 /- Unit test for [iter_adapters::test_range_inclusive_empty] -/
-#assert (test_range_inclusive_empty == ok ())
+#assert (test_range_inclusive_empty).reducesTo ()
 
 end iter_adapters
